\documentclass{article}

\usepackage{header}
%%%%%%%%%%%%%%%%%%%%%%%%%%%%%%%%%%%%%%%%%%%%%%%%%%%%%%%%
%Preamble

\title{Boundary Value Problems in Linear PDEs Example Sheet 1}
\author{Linden Disney-Hogg}
\date{December 2018}

%%%%%%%%%%%%%%%%%%%%%%%%%%%%%%%%%%%%%%%%%%%%%%%%%%%%%%%%
%%%%%%%%%%%%%%%%%%%%%%%%%%%%%%%%%%%%%%%%%%%%%%%%%%%%%%%%
\begin{document}

\maketitle
\tableofcontents

%%%%%%%%%%%%%%%%%%%%%%%%%%%%%%%%%%%%%%%%%%
%%%%%%%%%%%%%%%%%%%%%%%%%%%%%%%%%%%%%%%%%%
\section{Question 1}

Let $q:\mbb{R}_{>0} \times [0,T] \to \mbb{R}$ satisfy 
\eq{
q_t &= q_{xx} \\
q|_{t=0} &= q_0 \\
q_x |_{x=0} &= g_1
}
Assume the boundary conditions are compatible, and that $q_0$ has sufficient decay.\\
Define $g_0 = q|_{x=0}$. Then we have the transforms for $\lambda \in \mbb{C}$
\eq{
\hat{q}(\lambda,t) &= \int_0^\infty e^{-i\lambda x} q(x,t) \, dx \\
\tilde{g}_j(\lambda,t) &= \int_0^t e^{\lambda \tau} g_j(t) \, dt
}
Note that convergence of the integrals mean that $\hat{q}$ is defined only for $\Re(-i\lambda) \leq 0 \Rightarrow \Im \lambda \leq 0$, but $\tilde{g}_j$ are defined on all of $\mbb{C}$. \\
We may now derive a global relation.
\eq{
\del_t \hat{q}(\lambda,t) &= \int_0^\infty e^{-i\lambda x} q_t(x,t) \, dx \\
&= \int_0^\infty e^{-i\lambda x} q_{xx}(x,t) \, dx \\
&= \psquare{e^{-i\lambda x} q_x(x,t)}_{x=0}^\infty - \int_0^\infty -i\lambda e^{-i\lambda x} q_x(x,t) \, dx \\
&= -g_1(t) + i\lambda \pbrace{\psquare{e^{-i\lambda x} q(x,t)}_0^\infty- \int_0^\infty -i\lambda e^{-i\lambda x} q(x,t) \, dx}\\
&= -g_1(t) - i\lambda g_0(t) - \lambda^2 \hat{q}(\lambda,t)
}
In these steps, we have used the domain on $\lambda$ and the niceness of $q$ to argue that the upper limits are 0. Hence 
\eq{
\del_t \pround{e^{\lambda^2 t} \hat{q}(\lambda,t)} &= -[g_1(t) + i\lambda g_0(t)] e^{\lambda^2 t} \\
\Rightarrow e^{\lambda^2 t}\hat{q}(\lambda,t) - \hat{q}_0(\lambda) &= -\int_0^t e^{\lambda^2 \tau} [g_1(\tau) + i\lambda g_0(\tau)] \, d\tau \\
\Rightarrow e^{\lambda^2 t} \hat{q}(\lambda,t) &= \hat{q}_0(\lambda) - [\tilde{g}_1(\lambda^2,t) + i\lambda \tilde{g}_0(\lambda^2,t)]
}
This global relation is defined on the Lower Half Plane (LHP). \\
Now using the Fourier inversion theorem 
\eq{
q(x,t) &= \frac{1}{2\pi} \int_{-\infty}^\infty e^{i\lambda x} \hat{q}(\lambda,t) \, d\lambda \\
&= \frac{1}{2\pi} \int_{-\infty}^\infty e^{i\lambda x - \lambda^2 t} \hat{q}_0(\lambda) \, d\lambda - \frac{1}{2\pi} \int_{-\infty}^\infty e^{i\lambda x - \lambda^2 t} [\tilde{g}_1(\lambda^2,t) + i\lambda \tilde{g}_0(\lambda^2,t)] \, d\lambda
}
We now wish to deform the second contour integral, as it will be convenient when we wish to remove $g_0$ from the solution. Note 
\eq{
e^{-\lambda^2 t }\tilde{g}_j(\lambda^2,t) &= \int_0^t e^{\lambda^2 (\tau-t)} g_j(\tau) \,d\tau \\
&= \psquare{\frac{e^{\lambda^2 (\tau-t)}}{\lambda^2} g_j(\tau)}_0^t - \int_0^t \frac{e^{\lambda^2 (\tau-t)}}{\lambda^2} g_j^{(1)}(\tau) \, d\tau \\
&= \frac{1}{\lambda^2}\psquare{g_j(t) - e^{-\lambda^2 t}g_j(0)} - \frac{1}{\lambda^4}\psquare{g_j^{(1)}(t) - e^{-\lambda^2 t}g_j^{(1)}(0)} + \dots 
}
so if $\Re \lambda^2 \geq 0$, $\tilde{g}_j(\lambda^2) = \mc{O}\pround{\frac{1}{\lambda^2}}$ as $\abs{\lambda}\to\infty$. Now we can deform the contour onto the contour in the UHP $\Re \lambda^2 = 0$. This is an application of Jordan's lemma (hence the requirement that we defrom in the UHP) and Cauchy's theorem. The contour can also be written $\del D^+$, where
\eq{
D^+ = \set{\lambda \in \mbb{C} : \Re\lambda^2 \leq 0, \Im \lambda \geq 0}
}
\eq{
\Rightarrow  q(x,t) = \frac{1}{2\pi} \int_{-\infty}^\infty e^{i\lambda x - \lambda^2 t} \hat{q}_0(\lambda) \, d\lambda - \frac{1}{2\pi} \int_{\del D^+} e^{i\lambda x - \lambda^2 t} [\tilde{g}_1(\lambda^2,t) + i\lambda \tilde{g}_0(\lambda^2,t)] \, d\lambda
}
We now recognise
\eq{
\int_0^t \dots dt = \int_0^T \dots dt - \int_t^T \dots dt
}
so we can write 
\eq{
\tilde{g}_j(\lambda^2,t) = \tilde{g}_j(\lambda^2,T) - \int_t^T e^{\lambda^2 \tau} g_j(\tau) \, d\tau
}
By the same argument as before 
\eq{
e^{-\lambda^2 t} \int_t^T e^{\lambda^2 \tau} g_j(\tau) \, d\tau = \mc{O}\pround{\frac{1}{\lambda^2}}
}
provided $\Re \lambda^2 \leq 0$. Hence we apply Jordan's lemma and Cauchy's theorem again to get 
\eq{
q(x,t) = \frac{1}{2\pi} \int_{-\infty}^\infty e^{i\lambda x - \lambda^2 t} \hat{q}_0(\lambda) \, d\lambda - \frac{1}{2\pi} \int_{\del D^+} e^{i\lambda x - \lambda^2 t} [\tilde{g}_1(\lambda^2) + i\lambda \tilde{g}_0(\lambda^2)] \, d\lambda
}
labelling $\tilde{g}_j(\lambda^2,T) = \tilde{g}_j(\lambda^2)$. \\
Recall now the global relation 
\eq{
e^{\lambda^2 t}\hat{q}(\lambda,t) = \hat{q}_0(\lambda) - \tilde{g}_1(\lambda^2,t) - i\lambda\tilde{g}_0(\lambda^2,t) \quad \Im\lambda \leq 0
}
By noting the symmetry $\lambda \to - \lambda$, we have the second global relation 
\eq{
e^{\lambda^2 t}\hat{q}(-\lambda,t) = \hat{q}_0(-\lambda) - \tilde{g}_1(\lambda^2,t) + i\lambda\tilde{g}_0(\lambda^2,t) \quad \Im\lambda \geq 0
}
This second global relation is valid along $\del D^+$, so we may substitute to give 
\eq{
q(x,t) = \frac{1}{2\pi} \int_{-\infty}^\infty e^{i\lambda x - \lambda^2 t} \hat{q}_0(\lambda) \, d\lambda - \frac{1}{2\pi} \int_{\del D^+} e^{i\lambda x - \lambda^2 t} [\tilde{g}_1(\lambda^2) + e^{\lambda^2 T}\hat{q}(-\lambda,T) - \hat{q}_0(-\lambda)+ \tilde{g}_1(\lambda^2)] \, d\lambda
}
As before, we may show 
\eq{
e^{\lambda^2 (T-t)} \hat{q}(-\lambda,T) = \mc{O}\pround{\frac{1}{\lambda}}
}
as $\abs{\lambda} \to \infty$ for $\Re\lambda^2 \leq 0$, so by Jordan's lemma and Cauchy's theorem we may say that the contribution og the $\hat{q}$ term in the integral is 0. We may then deform back the $\hat{q}_0$ contour to give 
\eq{
q(x,t) = \frac{1}{2\pi} \int_{-\infty}^\infty e^{i\lambda x - \lambda^2 t} \psquare{\hat{q}_0(\lambda) + \hat{q}_0(-\lambda)} \,d\lambda - \frac{1}{\pi}\int_{\del D^+} e^{i\lambda x - \lambda^2 t} \tilde{g}_1(\lambda^2) \, d\lambda
}
To verify that this is the solution, not that because all the $x$ and $t$ dependence is in the exponentials, certainly the solution obeys the PDE. Moreover, evaluating at $t=0$ we may use Jordan's lemma and Cauchy's theorem to remove the contribution from $\hat{q}_0(-\lambda)$ and $\tilde{g}_1$. What remains is the inverse FT of $\hat{q}_0$, as desired. In the case of $x=0$, once the derivative is taken the first integral cancels by symmetry. Parametrising $\del D^+$ as $\lambda^2 = is$ yields $g_1(t)$ in the latter integral. 

%%%%%%%%%%%%%%%%%%%%%%%%%%%%%%%%%%%%%%%%%%
%%%%%%%%%%%%%%%%%%%%%%%%%%%%%%%%%%%%%%%%%%
\section{Question 2}

%%%%%%%%%%%%%%%%%%%%%%%%%%%%%%%%%%%%%%%%%%
%%%%%%%%%%%%%%%%%%%%%%%%%%%%%%%%%%%%%%%%%%
\section{Question 3}
Let $q:\mbb{R}_{>0} \times [0,T] \to \mbb{R}$ satisfy the IBVP 
\eq{
q_t &= -q_{xxx}-q_x \\
q|_{t=0} &= q_0 \\
q |_{x=0} &= g_0
}
with compatibility and decay conditions. Preemptively defining 
\eq{
\omega(\lambda) = (i\lambda)^3 + (i\lambda) = i\lambda(1 - \lambda^2)
}
we can derive the global relation 
\eq{
\del_t \hat{q}(\lambda,t) &= g_2(t) +i \lambda g_1(t) +(i\lambda)^2 g_0(t) - (i\lambda)^3 \hat{q}(\lambda,t) + g_0(t) - (i\lambda)\hat{q}(\lambda,t) \\
\Rightarrow  e^{\omega(\lambda)t} \hat{q}(\lambda,t) &= \hat{q}_0(\lambda) + \psquare{\tilde{g}_2(\omega(\lambda),t) + i\lambda \tilde{g}_1(\omega(\lambda),t) + (1-\lambda^2)\tilde{g}_0(\omega(\lambda),t)}
}
valid in the LHP. Again we may invert this to get 
\eq{
q(x,t) = \frac{1}{2\pi} \int_{\mbb{R}} e^{i\lambda x - \omega(\lambda)t} \hat{q}_0(\lambda) \, d\lambda + \frac{1}{2\pi} \int_{\mbb{R}} e^{i\lambda x - \omega(\lambda)t} \psquare{\tilde{g}_2(\omega(\lambda),t) + i\lambda \tilde{g}_1(\omega(\lambda),t) + (1-\lambda^2)\tilde{g}_0(\omega(\lambda),t)} \, d\lambda 
}
If we define 
\eq{
D^+ = \set{\lambda \in \mbb{C} : \Re \omega(\lambda) \leq 0 , \Im\lambda > 0}
}
then we may deform the contour of the $\tilde{g}$ terms by the same argument as before onto $\del D^+$. We now seek solutions $\nu(\lambda)$ to the equation 
\eq{
\omega(\nu(\lambda)) &= \omega(\lambda) \\
\Rightarrow \nu(\lambda)^3 - \nu(\lambda) &= \lambda^3 - \lambda \\
\Rightarrow 0 &= (\nu(\lambda) - \lambda)(\nu(\lambda)^2+\lambda \nu(\lambda) + \lambda^2-1)
}
Note that $\nu(\lambda) = \lambda$ must always be a solution to this equation. Label the other two roots $\nu_1, \nu_2$, which can be seen to be distinct from the quadratic (i.e. look at $b^2 - 4ac = \lambda^2 - 4(\lambda^2-1) = 4-3\lambda^2$). Note we have the helpful relations 
\eq{
\nu_1 + \nu_2 &= -\lambda \\
\nu_1 \nu_2 &= \lambda^2 - 1
}
As $\omega(\lambda)$ is cubic with 3 distinct roots, the condition $\Re\omega(\lambda) \leq 0$ must define three regions. Moreover, as $\lambda \in \mbb{R} \Rightarrow \omega(\lambda) \in \mbb{I}$. Further thinking/drawing shows that $D^+$ is one of these regions, so the maps $\lambda \to \nu_1, \lambda \to \nu_2$ must permute the regions. Hence we get two more GRs 
\eq{
e^{\omega(\lambda)t} \hat{q}(\nu_j,t) &= \hat{q}_0(\nu_j) + \psquare{\tilde{g}_2(\omega(\lambda),t) + i\nu_j \tilde{g}_1(\omega(\lambda),t) + (1-\nu_j^2)\tilde{g}_0(\omega(\lambda),t)} 
}
Both of these two equations must be valid on $\del D^+$ as $\nu(\lambda)$ must end up in the LHP under the transform. Moreover, as a result, the $\hat{q}$ terms will give 0 contribution over the integral region as $\Im \nu(\lambda) \leq 0$, so in the following algebra we may preemptively set the term to zero (note therefore the equalities do not hold exactly, but more precisely as an equivalence relation under the integral). Hence
\eq{
(\nu_1 - \nu_2)\tilde{g}_2 &= -\psquare{\nu_1 \hat{q}_0(\nu_2) - \nu_2 \hat{q}_0(\nu_1)} - \psquare{\nu_1(1-\nu_2^2) - \nu_2(1-\nu_1^2)} \tilde{g}_0 \\
&= \psquare{\nu_2 \hat{q}_0(\nu_1) - \nu_1 \hat{q}_0(\nu_2)} - \psquare{(\nu_1 - \nu_2)(1 + \nu_1 \nu_2) } \tilde{g}_0 \\
\Rightarrow \tilde{g}_2 &= \frac{\nu_2 \hat{q}_0(\nu_1) - \nu_1 \hat{q}_0(\nu_2)}{\nu_1 - \nu_2} - \lambda^2 \tilde{g}_0
}
and 
\eq{
i(\nu_1 - \nu_2)\tilde{g}_1 &= -\psquare{\hat{q}_0(\nu_1) - \hat{q}_0(\nu_2)} - \psquare{(1-\nu_1^2) - (1-\nu_2^2)} \tilde{g}_0 \\ 
\Rightarrow i \tilde{g}_1 &= \frac{\hat{q}_0(\nu_2) - \hat{q}_0(\nu_1)}{\nu_1 - \nu_2} + (\nu_1 + \nu_2) \tilde{g}_0 \\
&= \frac{\hat{q}_0(\nu_2) - \hat{q}_0(\nu_1)}{\nu_1 - \nu_2} - \lambda \tilde{g}_0
}
Substituting yields 
\eq{
q(x,t) =&  \frac{1}{2\pi} \int_{\mbb{R}} e^{i\lambda x - \omega(\lambda)t} \hat{q}_0(\lambda) \, d\lambda \\
& + \frac{1}{2\pi} \int_{\del D^+} e^{i\lambda x - \omega(\lambda)t} \psquare{\frac{(\nu_2-\lambda) \hat{q}_0(\nu_1) - (\nu_1 - \lambda) \hat{q}_0(\nu_2)}{\nu_1 - \nu_2} + (1-3\lambda^2)\tilde{g}_0(\omega(\lambda),t)} \, d\lambda
}

\subsection{2009, Question 1, part (d)}
This same problem, now with infinite time domain, came up in the 2009 paper, question 1. Part (d) asked for verification that the problem solved the IBVP. 

\subsubsection{Solve the PDE}

\subsubsection{}
\end{document}